\documentclass[a4paper,11pt]{article}

\usepackage{mathpartir}
\usepackage{amsmath,amsthm,amsfonts}
\usepackage{ amssymb }
\usepackage{color}
\usepackage{algorithm}
\usepackage{algorithmic}
\usepackage{microtype}


\input{ldefs}
\input{prelude}
\newcommand{\aexpr}{a}
\newcommand{\bexpr}{b}
\newcommand{\cmd}{c}
\newcommand{\node}{N}
\newcommand{\assign}[2]{ \mathrel{ #1  \leftarrow #2 } }
\newcommand{\fassign}[3]{ \mathrel{ #1  \leftarrow^{#3}  \delta^{#3}(
    #2 ) } }
\newcommand{\impif}[3]{\mathrel{\eif \eapp #1\eapp \ethen \eapp #2 \eapp
    \eelse \eapp #3 }}
\newcommand{\impwhile}[2]{\mathrel{ \kw{while} (#1) \eapp #2 } }
\newcommand{\labl}{l}

\let\originalleft\left
\let\originalright\right
\renewcommand{\left}{\mathopen{}\mathclose\bgroup\originalleft}
\renewcommand{\right}{\aftergroup\egroup\originalright}

\theoremstyle{definition}

\title{Clairvoyant Semantics for Adaptivity Analysis}

\author{}

\date{}

\begin{document}

\maketitle



\[\begin{array}{llll}
    \mbox{Pure Expr.} & \expr & ::= & \econst ~|~ x ~|~ \expr \eapp \expr 
                                      ~|~ \lambda x. \expr  ~|~ \efix
                                      \, f(x) \, \expr ~|~
                                      \epair{\expr}{\expr} ~|~
                                      \eprojl\, \expr ~|~ \eprojr\, \expr\\ 
                      & & &  \etrue ~|~ \efalse ~|~ \eif (\expr, \expr
                            , \expr)  ~|~ \enil ~|~ \expr \,  \econs
                            \, \expr ~|~  \emonadic{m} \\
    % 
    \mbox{Monadic Expr.} & \mexpr & ::= & \mreturn(\expr) ~|~
                                          \mlet{x}{\expr}{\mexpr} ~|~
                                         \mpair{\mexpr}{\mexpr} ~|~ \eop(\mexpr)\\
    %
    \mbox{Value.} & v & ::= & \econst ~|~ \lambda x. \expr ~|~ \pair{\valr_1}{\valr_2} ~|~  \etrue ~|~ \efalse  ~|~ \emonadic{m}\\
    %
    \mbox{Types} & \type &::=  &  \tbase ~|~ \type \to \type ~|~ \type
                                 \times \type
                                 ~|~ \tmonad(\type)  \\
  \end{array}\]



\begin{definition}
  Let $\vdash \mexpr : \tmonad(\type)$, its \emph{adaptivity} is defined as:
  $$
  \min\{\adapt ~|~ \exists \expr',\valr. \mexpr\bigstepf{\adapt} \expr' \land \expr' \bigstep \valr \}
  $$
\end{definition}


\begin{figure}[h]
  \begin{mathpar}
    \inferrule{}{
     \tctx, x:\type \vdash x :  \type
    }~\textbf{ST-AX}
    %
    \and
    %
    \inferrule{
    }{
      \tctx \vdash c: \tbase
    }~\textbf{ST-CST}   
    \and
    %
    \inferrule{
      \tctx, x: \type_1 \vdash \expr : \type_2
    }{
     \tctx \vdash \lambda x. \expr  :\type_1 \to \type_2
    }~\textbf{ST-LAM}
    \and
    %
    \inferrule{
       \tctx \vdash\expr_1:  \type_1 \to \type_2      \\
      \tctx \vdash\expr_2 : \type_1
    }{
      \tctx \vdash ( \expr_1 \eapp \expr_2) : \type_2
    }~\textbf{ST-app}
    %
    \\
    ....
  \end{mathpar}
  \caption{Simple Types - pure rules}
  \label{fig:simple-types-pure}
\end{figure}

 \begin{figure}[h]
  \begin{mathpar}
    \inferrule{
      \tctx \vdash \expr :  \type
    }{
     \tctx \vdash \return(\expr) : \tmonad( \type)
    }~\textbf{ST-RET}
    %
    \and
    %
    \inferrule{
      \tctx \vdash \expr :  \tmonad(\type_1)
      \\
      \tctx, x: \type_1 \vdash \mexpr :  \tmonad(\type_2)
    }{
      \tctx \vdash \mlet{\expr}{x}{\mexpr} : \tmonad(\type_2)
    }~\textbf{ST-LET}
    %
    \and
    %
    \inferrule{
      \tctx \vdash \expr  :  \tmonad({\tt row})
      \\
      \hat{\delta}:{\tt row} \to [0,1]
   }{  \tctx \vdash \delta(\expr) : \tmonad([0,1])
    }~\textbf{ST-DELTA}
  \end{mathpar}
  \caption{Simple Types - monadic rules}
  \label{fig:simple-types-monadic}
\end{figure}


\begin{figure}[h]
  \begin{mathpar}
    \inferrule{
    }{
     \valr \bigstep \valr } ~\textsf{S-VAL}
   \and
   %
   \and
  %
  \inferrule{
    \expr_1 \bigstep \lambda x.\expr  \\
     \expr_2 \bigstep \valr_2  \\
   \expr[\valr_2/x] \bigstep \valr_3
  }{
     \expr_1 \eapp \expr_2 \bigstep \valr_3
   }~\textsf{S-APP}
    %
  \and
 %
 \inferrule{
  \expr_1 \bigstep  \etrue
   \\
   \expr_2  \bigstep \valr_2
  }{
   \env, \eif (\expr_1 ,\expr_2 , \expr_3) \bigstep \valr_2
  }~\textsf{S-IFT}
\and
 \inferrule{
  \expr_1 \bigstep \etrue
   \\
   \expr_3  \bigstep \valr_3
  }{
   \eif (\expr_1 ,\expr_2 , \expr_3) \bigstep  \valr_3
  }~\textsf{S-IFF}
  % %
 %
  \and
  %
  \inferrule{
     \expr_1  \bigstep \valr_1 \\
     \expr_2  \bigstep \valr_2 \\
  }{
   \pair{\expr_1}{\expr_2} \bigstep
   \pair{\valr_1}{\valr_2}
 }~\textsf{S-PROD}
 %
  \and
  %
  \inferrule{
    \expr  \bigstep (\valr_1, \valr_2) 
  }{
   \eprojl{\, \expr} \bigstep \valr_1
 }~\textsf{S-PL}
 %
  \and
  %
  \inferrule{
    \expr  \bigstep (\valr_1, \valr_2) 
  }{
   \eprojr{(\expr)} \bigstep \valr_2
 }~\textsf{S-PR}
\end{mathpar}
  \caption{Big-step semantics, pure  rules.}
  \label{fig:semantics-pure}
\end{figure}


\begin{figure}[h]
  \begin{mathpar}
    \inferrule{
    }{
     \return(\expr) \bigstepf{0} \expr } ~\textsf{FS-RET}
   \and
   %
  \inferrule{
    \expr\bigstep \emonadic{\mexpr_1}  \\
     \mexpr_1\bigstepf{\adapt_1} \expr_1  \\
     \mexpr[\expr_1/x] \bigstepf{\adapt_2} \expr_2  \\
  }{
     \mlet{x}{\expr}{\mexpr} \bigstepf{\adapt_1+\adapt_2} \expr_2
   }~\textsf{FS-BIND}
    %
 \and
   %
  \inferrule{
     \mexpr\bigstepf{\adapt_2} \expr_2  \\
   }{
     \mlet{x}{\expr_1}{\mexpr} \bigstepf{\adapt_2} \expr_2
   }~\textsf{FS-SKIP}
   \and
  \inferrule{
    \mexpr \bigstepf{\adapt} \expr  \\
    \expr \bigstep \valr\\
    \hat{\eop}(\valr)=\valr'
  }{
     \eop(\mexpr)  \bigstepf{\adapt+1} \valr'
   }~\textsf{FS-MECH}
   %
  \and
  %
  \inferrule{
     \mexpr_1  \bigstepf{\adapt_1} \expr_1 \\
     \mexpr_2  \bigstepf{\adapt_2} \expr_2 \\
  }{
   \mpair{\mexpr_1}{\mexpr_2} \bigstep
   \pair{\expr_1}{\expr_2}
 }~\textsf{FS-PROD}
\end{mathpar}
  \caption{Big-step semantics, forcing rules.}
  \label{fig:semantics-forcing}
\end{figure}



\begin{figure}[h]
  \begin{mathpar}
    \inferrule{}{
     \tctx, x:!_1\type \vdash x :  \type
    }~\textbf{ST-AX}
    %
    \and
    %
    \inferrule{
    }{
      \tctx \vdash c: \tbase
    }~\textbf{ST-CST}   
    \and
    %
    \inferrule{
      \tctx, x: !_i \type_1 \vdash \expr : \type_2
    }{
     \tctx \vdash \lambda x. \expr  :!_i \type_1 \to \type_2
    }~\textbf{ST-LAM}
    \and
    %
    \inferrule{
       \tctx_1 \vdash\expr_1:  !_i\type_1 \to \type_2      \\
      \tctx_2 \vdash\expr_2 : \type_1
    }{
      \tctx_1+i*\tctx_2 \vdash ( \expr_1 \eapp \expr_2) : \type_2
    }~\textbf{ST-app}
    %
    \\
    ....
  \end{mathpar}
  \caption{Simple Types - pure rules}
  \label{fig:simple-types-pure}
\end{figure}

 \begin{figure}[h]
  \begin{mathpar}
    \inferrule{
      \tctx \vdash \expr :  \type
    }{
     \tctx \vdash \return(\expr) : \tmonad( \type)
    }~\textbf{ST-RET}
    %
    \and
    %
    \inferrule{
      \tctx \vdash \expr :  \tmonad(\type_1)
      \\
      \tctx, x: \type_1 \vdash \mexpr :  \tmonad(\type_2)
    }{
      \tctx \vdash \mlet{\expr}{x}{\mexpr} : \tmonad(\type_2)
    }~\textbf{ST-LET}
    %
    \and
    %
    \inferrule{
      \tctx \vdash \expr  :  \tmonad({\tt row})
      \\
      \hat{\delta}:{\tt row} \to [0,1]
   }{  \tctx \vdash \delta(\expr) : \tmonad([0,1])
    }~\textbf{ST-DELTA}
  \end{mathpar}
  \caption{Simple Types - monadic rules}
  \label{fig:simple-types-monadic}
\end{figure}

\clearpage
\section{Example}
1. A mechnism with the simple input query : $\lambda x. \emonadic{
  \eop(\mreturn(x)) } \eapp b \bigstep \emonadic{\eop(\mreturn(b))} $.\\
2. A mechnism with a complex input query : $\lambda x. \emonadic{
  \eop(\mreturn(x)) } \eapp \emonadic{\eop(\mreturn(b))} \bigstep
\emonadic{\eop(\mreturn( \eop(\mreturn(b)) ))} $.\\
3. A mechnism with more arguments : \\
 $ \lambda x. \lambda y. \emonadic{ \mlet{z}{
     \emonadic{\eop(\mreturn(x))}  }{   \eop( \mreturn{ (\eprojl{y} +
       z) }  )   } }  \eapp b \eapp (b_1, b_2)$\\
 4.  A mechnism with impure arguments : \\
 $ \lambda x. \lambda y. \emonadic{ \mlet{z}{
     x }{   \eop( \mreturn{ (\eprojl{y} + z) }  )   } } \eapp
 \emonadic{\eop(\mreturn(b))} \eapp \epair{b_1}{b_2} $.\\
5.  A mechnism with impure pair : \\
 $ \lambda x. \lambda y. \emonadic{ \mlet{z}{
     x }{
     \mlet{n}{y}{
     \eop( \mreturn{ (\eprojl{n} + z) }  ) }   }
 } \eapp$ \\
 $\emonadic{\eop(\mreturn(b))} \eapp \emonadic{\mpair{ \mreturn( b_1)}{
    \eop( \mreturn( b_2) ) } }$.\\
6. two rounds\\
$\efix \, f(j) \, \lambda \, k.  $\\
$ \eif ( j < k , $\\
$\emonadic{ \mlet{a}{ \emonadic{\eop (\mreturn(l+k) ) }
  } { \mlet{t'}{f \eapp (j+1) \eapp k }{  \mreturn( (a, j) \econs t' )  } } } ,   $\\
$ \emonadic{ \mreturn ( \enil )  } ) $\\
\end{document}



