\begin{example}
 \[
 \begin{array}{ll}
 & \sem{
 \ewhile {}^0 (x > 0) {}^1 x = x - 1;
 } \triangleq \\
 & \left\{ \left< \pi_1^0, ^0\right> \mid \pi_1^0 \in \mathbb{T^{+}} \right\}
 \\
 \cup & \left\{ \left< \pi_1^0, {}^0 \xrightarrow{(x > 0)} {}^1 \xrightarrow{(x = x - 1) = v} {}^0 \right> 
 \mid \pi_i^0 \in \mathbb{T^{+}} \land 
 \sem{(x > 0)}\env(\pi_1^0) = \etrue  \land
 \sem{(x - 1)}\env(\pi_1^0 \xrightarrow{(x > 0)} {}^1) = v \right\}
 \\
 \cup & \left\{ \left< \pi_1^0, {}^0 \xrightarrow{(x > 0)} {}^1 \xrightarrow{(x = x - 1) = v_1} {}^0 \xrightarrow{(x > 0)} {}^1 \xrightarrow{(x = x - 1) = v_2} {}^0 \right> 
 \left \vert 
 \begin{array}{l}
 \pi_i^0 \in \mathbb{T^{+}} \\
 \land 
 \sem{(x > 0)}\env(\pi_1^0) = \etrue  \\
 \land
 \sem{(x - 1)}\env(\pi_1^0 \xrightarrow{(x > 0)} {}^1) = v_1 \\
 \land 
 \sem{(x > 0)}\env(\pi_1{}^0 \xrightarrow{(x > 0)} {}^1 \xrightarrow{(x = x - 1) = v_1} {}^0) = \etrue \\
 \land
 \sem{(x - 1)}\env(\pi_1^0 \xrightarrow{(x > 0)} {}^1 \xrightarrow{(x = x - 1) = v_1} {}^0 \xrightarrow{(x > 0)} {}^1) = v_2
 \end{array}
 \right.
 \right\}
 \\
 \cup & \cdots 
 \\
 \cup & \left\{ \left< \pi_1^0, {}^0 \xrightarrow{(x > 0)} {}^1\xrightarrow{(x = x - 1) = v_1} {}^0 \cdots  {}^0 \xrightarrow{\neg(x > 0)} {}^l \right>  
 \left \vert 
 \begin{array}{l}
 \pi_1^0 \in \mathbb{T^{+}}\\
 \land 
 \sem{(x > 0)}\env(\pi_1^0) = \etrue  \\
 \land
 \sem{(x - 1)}\env(\pi_1^0 \xrightarrow{(x > 0)} {}^1) = v_1 \\
 \land \cdots \\
 % \land
 % \sem{(x - 1)}\env(\pi_1^0 \xrightarrow{(x > 0)} {}^1 \xrightarrow{(x = x - 1) = v} {}^0 \xrightarrow{(x > 0)} {}^1) = v_2\\
 \land 
 \sem{(x > 0)}\env(\pi_i{}^0 \xrightarrow{(x > 0)} {}^1\xrightarrow{(x = x - 1) = v_1} {}^0 \cdots  {}^0) = \efalse \\
 \land l = \kw{aft}[\ewhile {}^0 (x > 0) {}^1 x = x - 1;]
 \end{array}
 \right.
 \right\}
 \end{array}
 \]
 \end{example}
 %
 \begin{example}
 \[
 \begin{array}{ll}
 & \sem{ 
 \epsilon {}^0 x = 1; \ewhile {}^1  (x > 0) {}^2 x = x - 1 ; {}^3 }  \\
 \triangleq & 
 \sem{\epsilon {}^0 x = 1;} 
 \cup
 \left\{ \left< \pi_1{}^0, {}^0\pi_2^1\pi_3^3\right> 
 \left \vert 
 \begin{array}{l}
 \left< \pi_1^0, {}^0\pi_2^1 \right> \in \sem{\epsilon {}^0 x = 1;}
 \\
 \land \left< \pi_1{}^0\pi_2^1, {}^1\pi_3^3\right>  \in 
 \sem{\ewhile {}^1 (x > 0) {}^2 x = x - 1 ;} 
 \end{array}
 \right.
 \right\}
 \\
 \triangleq & 
 \sem{\epsilon}
 \cup
 \left\{ \left< \pi_1{}^0, {}^0 \pi_2 {}^1 \right> 
 \left \vert 
 \begin{array}{l}
 \left< \pi_1{}^0, {}^0 \right> \in \sem{\epsilon}  \land \\
  
 \left< \pi_1{}^0, {}^0 \pi_2{}^1 \right> \in \sem{ {}^0 x = 1;}
 \end{array}
 \right.
 \right\}
 \cup
 \left\{ \left< \pi_1{}^0, {}^0\pi_2^1\pi_3 {}^3\right> 
 \left \vert 
 \begin{array}{l}
 \left< \pi_1{}^0, {}^0\pi_2^1 \right> \in \sem{\epsilon {}^0 x = 1;}\land
 \\
  \left< \pi_1 {}^0\pi_2 {}^1, {}^1 \pi_3 {}^3\right>  \in 
 \sem{\ewhile {}^1  (x > 0) {}^2 x = x - 1 ;} 
 \end{array}
 \right.
 \right\}
 \\
 \triangleq 
 & \left\{ \left< \pi_1^0, ^0\right> \mid \pi_1^0 \in \mathbb{T^{+}} \right\} \\
 & \cup
 \left\{ \left< \pi_1{}^0, {}^0 \xrightarrow{(x = 1) = 1} {}^1\right> 
 \vert 
 \pi_1^0 \in \mathbb{T^{+}}
 \land 
 \sem{1}\env(\pi_1^0) = 1
 \right\} \\
 & \cup
 \left\{ \left< \pi_1{}^0, {}^0\xrightarrow{(x = 1) = 1} {}^1\pi_3^3\right> 
 \left \vert 
 % \begin{array}{l}
 \pi_1^0 \in \mathbb{T^{+}}
 \land
 \left< \pi_1 {}^0\xrightarrow{(x = 1) = 1} {}^1, {}^1\pi_3^3\right>  \in 
 \sem{\ewhile {}^1  (x > 0) {}^2 x = x - 1 ; {}^3} 
 % \end{array}
 \right.
 \right\}
 \\
 \triangleq
 & \left\{ \left< \pi_1^0, ^0\right> \mid \pi_1^0 \in \mathbb{T^{+}} \right\} \\
 & \cup
 \left\{ \left< \pi_1{}^0, {}^0 \xrightarrow{(x = 1) = 1} {}^1\right> 
 \vert 
 \pi_1^0 \in \mathbb{T^{+}}
 \land 
 \sem{1}\env(\pi_1^0) = 1
 \right\} 
 \\
 & \cup \left\{ \left< \pi_1^0, {}^0 \xrightarrow{(x = 1) = 1} {}^1 \xrightarrow{(x > 0)} {}^2 \xrightarrow{(x = x - 1) = 0} {}^1 \right> 
 \left \vert
 \begin{array}{l}
 \pi_i^0 \in \mathbb{T^{+}} \\
 \land 
 \sem{(x > 0)}\env(\pi_1{}^0 \xrightarrow{(x = 1) = 1} {}^1) = \etrue  \\
 \land
 \sem{(x - 1)}\env(\pi_1{}^0 \xrightarrow{(x = 1) = 1} {}^1 \xrightarrow{(x > 0)} {}^2) = 0
 \end{array}
 \right.
 \right\}
 \\
 & \cup \left\{ \left< \pi_1^0, {}^0 \xrightarrow{(x = 1) = 1} {}^1 \xrightarrow{(x > 0)} {}^2 \xrightarrow{(x = x - 1) = 0} {}^1 
 \xrightarrow{\neg(x > 0)} {}^3 \right> 
 \left \vert
 \begin{array}{l}
 \pi_i^0 \in \mathbb{T^{+}} \\
 \land 
 \sem{(x > 0)}\env(\pi_1{}^0 \xrightarrow{(x = 1) = 1} {}^1) = \etrue  \\
 \land
 \sem{(x - 1)}\env(\pi_1{}^0 \xrightarrow{(x = 1) = 1} {}^1 \xrightarrow{(x > 0)} {}^2) = 0 \\
 \land 
 \sem{(x > 0 )}\env(\pi_1{}^0 \xrightarrow{(x = 1) = 1} {}^1 \xrightarrow{(x > 0)} {}^2 \xrightarrow{(x = x - 1) = 0} {}^1) = \efalse
 \end{array}
 \right.
 \right\}
 \\
 \triangleq
 & \left\{ \left< \pi_1^0, ^0\right> \mid \pi_1^0 \in \mathbb{T^{+}} \right\} 
  \cup
 \left\{ \left< \pi_1{}^0, {}^0 \xrightarrow{(x = 1) = 1} {}^1\right> 
 \vert 
 \pi_1^0 \in \mathbb{T^{+}}
 \right\} 
  \cup \left\{ \left< \pi_1^0, {}^0 \xrightarrow{(x = 1) = 1} {}^1 \xrightarrow{(x > 0)} {}^2 \xrightarrow{(x = x - 1) = 0} {}^1 \right> 
 \vert \pi_i^0 \in \mathbb{T^{+}}
 \right\}
 \\
 & \cup \left\{ \left< \pi_1^0, {}^0 \xrightarrow{(x = 1) = 1} {}^1 \xrightarrow{(x > 0)} {}^2 \xrightarrow{(x = x - 1) = 0} {}^1 
 \xrightarrow{\neg(x > 0)} {}^3 \right> 
 \vert \pi_i^0 \in \mathbb{T^{+}}
 \right\}
 \end{array}
 \]
 \end{example}
 %
 \clearpage
 \begin{example}[Formal Example for Exclusion of Timing Channel].
 \label{ex:excltiming}
 \\
 $\mathsf{diff}(\omega, \omega')$ (in \cite{cousot2019abstract} Equation~(2)) excludes timing channel,(i.e., $\omega$ is a strict prefix of $\omega'$). There is an example showing this exclusion: 
 \[
 	\ewhile {}^1 (x > 0) \{{}^2 x = x - 1; {}^3 y = 1;\} 
 \]
 In this example, $y$'s execution times relies on value of $x$. Under the adaptivity scenario, $y$ depends on $x$ (control dependency).
 However, according to value dependency defined in Definition~2 \cite{cousot2019abstract}, we can never derive :
 \[
 	x \rightsquigarrow^{1}_{\ewhile {}^1 (x > 0) \{{}^2 x = x - 1; {}^3 y = 1;\}} y
 \]
 %
 \begin{proof}
 By semantics definition, we have:
 %
 \begin{equation}
 \label{eq:sem_timingdep}
 	\begin{array}{ll}
 & \sem{
 \ewhile {}^1 (x > 0) \{{}^2 x = x - 1; {}^3 y = 1;\} 
 } \triangleq \\
 & \left\{ \left< \pi_1^1, ^1\right> \mid \pi_1^1 \in \mathbb{T^{+}} \right\}
 \\
 \cup & \left\{ \left< \pi_1^1, {}^1 \xrightarrow{(x > 0)} {}^2 \xrightarrow{(x = x - 1) = v} {}^3 \xrightarrow{(y = 1) = 1} {}^1 \right> 
 \mid \pi_i^1 \in \mathbb{T^{+}} \land 
 \sem{(x > 0)}\env(\pi_1^1) = \etrue  \land
 \sem{(x - 1)}\env(\pi_1^1 \xrightarrow{(x > 0)} {}^2) = v\right\}
 \\
 \cup & \left\{ 
 \begin{array}{l}
 \left< \pi_1^1, {}^1 \xrightarrow{(x > 0)} {}^2 \xrightarrow{(x = x - 1) = v_1} {}^3 \xrightarrow{(y = 1) = 1} {}^1 \xrightarrow{(x > 0)} {}^2 \xrightarrow{(x = x - 1) = v_2} {}^3 \xrightarrow{(y = 1) = 1} {}^1 \right> 
  \\
  \left \vert
 \begin{array}{l}
 \pi_i^1 \in \mathbb{T^{+}} \\
 \land 
 \sem{(x > 0)}\env(\pi_1^1) = \etrue  \\
 \land
 \sem{(x - 1)}\env(\pi_1^1 \xrightarrow{(x > 0)} {}^2) = v_1 \\
 \land 
 \sem{(x > 0)}\env(\pi_1{}^1 \xrightarrow{(x > 0)} {}^2 \xrightarrow{(x = x - 1) = v_1} {}^3 \xrightarrow{(y = 1) = 1} {}^1) = \etrue \\
 \land
 \sem{(x - 1)}\env(\pi_1^1 \xrightarrow{(x > 0)} {}^2 \xrightarrow{(x = x - 1) = v_1} {}^3 \xrightarrow{(y = 1) = 1}
  {}^1 \xrightarrow{(x > 0)} {}^2) = v_2
 \end{array}
 \right.
 \end{array}
 \right\}
 \\
 \cup & \cdots 
 \\
 \cup & \left\{ 
 \begin{array}{l}
 \left< \pi_1^1, {}^1 \xrightarrow{(x > 0)} {}^2\xrightarrow{(x = x - 1) = v_1} {}^3 \xrightarrow{(y = 1) = 1} {}^1 \cdots  {}^1 \xrightarrow{\neg(x > 0)} {}^l \right>  
 \\
 \left \vert 
 \begin{array}{l}
 \pi_1^1 \in \mathbb{T^{+}}\\
 \land 
 \sem{(x > 0)}\env(\pi_1^1) = \etrue  \\
 \land
 \sem{(x - 1)}\env(\pi_1^1 \xrightarrow{(x > 0)} {}^2) = v_1 \\
 \land \cdots \\
 \land 
 \sem{(x > 0)}\env(\pi_i{}^1 \xrightarrow{(x > 0)} {}^2\xrightarrow{(x = x - 1) = v_1} {}^3 \xrightarrow{(y = 1) = 1} {}^1 \cdots  {}^1) = \efalse \\
 \land l = \kw{aft}[\ewhile {}^1 (x > 0) \{ {}^2 x = x - 1; {}^3 y = 1 \}]
 \end{array}
 \right.
 \end{array}
 \right\}
 \end{array}
 \end{equation}
 %
 %
 %
 Let $\pi_1^1, \pi_1'^1 \in \mathbb{T^{+}}$ be arbitrary traces s.t. 
 %
 $$\forall z \in \mathbb{V}\setminus \{x\}. ~ \env(\pi_1^1)(z) = \env(\pi_1'^1) $$ 
 %
 Let $v = \env(\pi_1^1)(x) $, $v' = \env(\pi_1'^1)(x')$, picking arbitrary $\pi_2, \pi_2'$ s.t.:
 \[
 	\left< \pi_1^1, \pi_2 \right>,  \left< \pi_1'^1, \pi'_2 \right> \in \sem{\ewhile {}^1 (x > 0) \{{}^2 x = x - 1; {}^3 y = 1;\} }
 \]
 %
 By Definition of $\mathsf{seqval}$, we have:
 \[
 	\mathsf{seqval}\sem{y}{}^2(\pi_1^1, \pi_2 ) = \underbrace{0 \cdots 1}_{0 \leq v}
 \]
 %
 \[
 	\mathsf{seqval}\sem{y}{}^2(\pi_1^1, \pi_2' ) = \underbrace{0 \cdots 1}_{0 \leq v'}
 \]
 %
  $\forall \omega_0, \omega_1', \omega_1, u, u' \st \underbrace{0 \cdots 1}_{0 \leq v} = \omega \cdot u \cdot \omega_1 \land \underbrace{0 \cdots 1}_{0 \leq v} = \omega \cdot u; \cdot \omega_1'$ we have:
 %
 \[
 	u = u' = 1
 \]
 %
 By $\mathsf{diff}(\omega, \omega')$ (in \cite{cousot2019abstract} Equation~(2) ), we have:
 %
 \[
 	\neg(\mathsf{diff}(\mathsf{seqval}\sem{y}{}^1(\pi_1^1, \pi_2 ), \mathsf{seqval}\sem{y}{}^1(\pi_1^1, \pi_2' )))
 \]
 %
 Then we have:
 \[
 \begin{array}{l}
 	\forall \left< \pi_1^1, \pi_2 \right>,  \left< \pi_1'^1, \pi'_2 \right> \in \mathcal{S}^{+\infty} \sem{\ewhile {}^2 (x > 0) {}^3 y = 1;} \st
 	\Big(
 	\forall z \in \mathbb{V}\setminus \{x\} \st \env(\pi_1^1)(z) = \env(\pi_1'^1) \st \\
 	\land \neg(\mathsf{diff}(\mathsf{seqval}\sem{y}{}^1(\pi_1^1, \pi_2 ), \mathsf{seqval}\sem{y}{}^1(\pi_1^1, \pi_2' )))\Big)
 \end{array}
 \] 
 \\
 %
 By Definition~2 (in \cite{cousot2019abstract}), 
 \[
 	\mathcal{S}^{+\infty}\sem{\ewhile {}^1 (x > 0) \{{}^2 x = x - 1; {}^3 y = 1;} 
 \notin \mathcal{D}^1(z, y)
 \]
 %
 By Definition~(4) (in \cite{cousot2019abstract}), we cannot derive:
 \[
 	x \rightsquigarrow^{1}_{\ewhile {}^1 (x > 0) \{{}^2 x = x - 1; {}^3 y = 1;\}} y
 \]
 %
 %
 \end{proof}
 \end{example}
 %
 \clearpage
 \begin{example}[Counter Example of Including Timing Channel].
 \label{ex:overapp}
 \\
 If $\mathsf{diff}(\omega, \omega')$ (in \cite{cousot2019abstract} Equation~(2)) simply includes timing channel,(i.e., $\omega$ is a strict prefix of $\omega'$) as follows:
 \[
 	\mathsf{diff}(\omega, \omega') \triangleq \exists \omega_0, \omega_1, \omega_1', v, v' 
 	\st \bigvee \left\{
 	\begin{array}{lr}
 	(\omega = \omega_0 \cdot v \omega_1
 		\land \omega' = \omega_0 \cdot v' \omega_1' \land v \neq v') & \mbox{original definition} \\
 	(\omega = \omega' \cdot v \cdot \omega_1) & \mbox{including timing channel} \\
 	\end{array}
 	\right\}
 \] 
 then by Definition~2 (in \cite{cousot2019abstract}), there is a over approximation example:
 \[
 	\ewhile {}^2 (x > 0) {}^3 y = 1; 
 \]
 Let $z \in \mathbb{V}\setminus \{x\}$ be arbitrary variable different from $x$,
 in this example, $y$ doesn't rely on $z$. 
 However, according to value dependency defined in Definition~2 \cite{cousot2019abstract} we can derive 
 \[
 	z \rightsquigarrow^{2}_{\ewhile {}^2 (x > 0) {}^3 y = 1;} y
 \]
 %
 \begin{proof}
 By semantics definition, we have:
 %
 \begin{equation}
 \label{eq:sem_timingoverapp}
 \begin{array}{ll}
 & \sem{ \ewhile {}^2 (x > 0) {}^3 y = 1; } \triangleq \\
 & \left\{ \left< \pi_1^2, ^2\right> \mid \pi_1^2 \in \mathbb{T^{+}} \right\}
 \\
 \cup & \left\{ \left< \pi_1^2, {}^2 \xrightarrow{(x > 0)} {}^3 \xrightarrow{(y = 1) = 1} {}^2 \right> 
 \mid \pi_i^2 \in \mathbb{T^{+}} \land 
 \sem{(x > 0)}\env(\pi_1^2) = \etrue  \land
 \sem{1}\env(\pi_1^2 \xrightarrow{(x > 0)} {}^3) = 1 \right\}
 \\
 \cup & \left\{ \left< \pi_1^2, {}^2 \xrightarrow{(x > 0)} {}^3 \xrightarrow{(y = 1) = 1} {}^2 \xrightarrow{(x > 0)} {}^3 \xrightarrow{(y = 1) = 1} {}^2 \right> 
 \left \vert 
 \begin{array}{l}
 \pi_i^2 \in \mathbb{T^{+}} \\
 \land 
 \sem{(x > 0)}\env(\pi_1^2) = \etrue  \\
 \land
 \sem{1}\env(\pi_1^2 \xrightarrow{(x > 0)} {}^3) = 1 \\
 \land 
 \sem{(x > 0)}\env(\pi_1{}^2 \xrightarrow{(x > 0)} {}^3 \xrightarrow{(y = 1) = 1} {}^2) = \etrue \\
 \land
 \sem{1}\env(\pi_1^2 \xrightarrow{(x > 0)} {}^3 \xrightarrow{(y = 1) = 1} {}^2 \xrightarrow{(x > 0)} {}^3) = 1
 \end{array}
 \right.
 \right\}
 \\
 \cup & \cdots 
 \\
 \cup & \left\{ \left< \pi_1^2, {}^2 \xrightarrow{(x > 0)} {}^3\xrightarrow{(x = x - 1) = v_1} {}^2 \cdots  {}^2 \xrightarrow{\neg(x > 0)} {}^l \right>  
 \left \vert 
 \begin{array}{l}
 \pi_1^2 \in \mathbb{T^{+}}\\
 \land 
 \sem{(x > 0)}\env(\pi_1^2) = \etrue  \\
 \land
 \sem{1}\env(\pi_1^2 \xrightarrow{(x > 0)} {}^3) = v_1 \\
 \land \cdots \\
 % \land
 % \sem{(x - 1)}\env(\pi_1^2 \xrightarrow{(x > 0)} {}^3 \xrightarrow{(x = x - 1) = v} {}^2 \xrightarrow{(x > 0)} {}^3) = v_2\\
 \land 
 \sem{(x > 0)}\env(\pi_i{}^2 \xrightarrow{(x > 0)} {}^3\xrightarrow{(y = 1) = 1} {}^2 \cdots {}^2) = \efalse \\
 \land l = \kw{aft}[\ewhile {}^2 (x > 0) {}^3 y = 1;]
 \end{array}
 \right.
 \right\}
 \end{array}
 \end{equation}
 %
 %
 Let $z \in \mathbb{V}\setminus \{x\}$ be arbitrary variable different from $x$,
 pick $\pi_0 = {}^0 \xrightarrow{z = 1} {}^1 \xrightarrow{x = 2} {}^2$, 
 $\pi_0' = {}^0 \xrightarrow{z = 2} {}^1 \xrightarrow{x = 2} {}^2$:
 \[
 	\left< \pi_0^2, {}^2 \xrightarrow{(x > 0)} {}^3 \xrightarrow{(y = 1) = 1} {}^2 \right> \in \sem{\ewhile {}^2 (x > 0) {}^3 y = 1;}
 \]
 %
 \[
 	\left< \pi_0'^2, {}^2 \xrightarrow{(x > 0)} {}^3 \xrightarrow{(y = 1) = 1} {}^2 \xrightarrow{(x > 0)} {}^3 \xrightarrow{(y = 1) = 1}{}^2\right> \in \sem{\ewhile {}^2 (x > 0) {}^3 y = 1; }
 \]
 %
 By Definition of $\mathsf{seqval}$, we have:
 \[
 	\mathsf{seqval}\sem{y}{}^2(\pi_0^2, {}^2 \xrightarrow{(x > 0)} {}^3 \xrightarrow{(y = 1) = 1} {}^2 ) = 1 \cdot
 \]
 %
 \[
 	\mathsf{seqval}\sem{y}{}^2(\pi_0'^2, {}^2 \xrightarrow{(x > 0)} {}^3 \xrightarrow{(y = 1) = 1} {}^2 \xrightarrow{(x > 0)} {}^3 \xrightarrow{(y = 1) = 1}{}^2 ) = 1 \cdot 1 \cdot
 \]
 %
 If $\mathsf{diff}(\omega, \omega')$ (in \cite{cousot2019abstract} Equation~(2) ) includes timing channel, i.e., 
 %
 \[
 	\mathsf{diff}(1 \cdot, 1 \cdot 1 \cdot) = \etrue
 \]
 %
 By Definition~2 (in \cite{cousot2019abstract}), 
 \[
 	\mathcal{S}^{+\infty}\sem{\ewhile {}^2 (x > 0) {}^3 y = 1;} 
 \in \mathcal{D}^2(z, y)
 \].
 %
 By Definition~(4) (in \cite{cousot2019abstract}):
 \[
 	z \rightsquigarrow^{2}_{\ewhile {}^2 (x > 0) {}^3 y = 1;} y
 \]
 %
 However, intuitively, the execution of $y$ doesn't relies on value of $z$ at all. This is a false positive example (or over approximation) of dependency.
 %
 \end{proof}
 \end{example}
 %
 \clearpage
 \clearpage
 \begin{example}[Approach-1 of Including Timing Channel]
 Modifying the Definition~2 (in \cite{cousot2019abstract}) as follows:
 \begin{defn}[Modified Data Dependency].
 \label{defn:mdfy_dep}
 \[
 	\begin{array}{lll}
 	\mathcal{D}^l(x, y) & \triangleq &
 	\Big\{ 
 	\Pi \in (\mathbb{T}^{+} \times \mathbb{T}^{+\infty})
 	\exists \config{\pi_1, \pi_2}, \config{\pi_1', \pi_2'} \in \Pi \st \\
 	&& \quad \big(
 	\forall z \in \mathbb{V}\setminus \{x\} \st \env(\pi_1)(z) = \env(\pi_1') \st \\
 	&& \quad  \quad \land \neg(\mathsf{diff}(\mathsf{seqval}\sem{y}{}^1(\pi_1, \pi_2 ), \mathsf{seqval}\sem{y}{}^1(\pi'_1, \pi_2')))
 	\big) \Big\} \\
 	& \cup & \Big\{ \Pi \in (\mathbb{T}^{+} \times \mathbb{T}^{+\infty})
 	\exists \config{\pi_1, \pi_2}, \config{\pi_1', \pi_2'} \in \Pi \st \forall \config{\pi_1', \pi_2''} \in \Pi\\
 	&& \quad \big(
 	\forall z \in \mathbb{V}\setminus \{x\} \st \env(\pi_1)(z) = \env(\pi_1') \st \\
 	&& \quad  \quad  \land |\mathsf{seqval}\sem{y}{}^1(\pi_1', \pi_2'')| \leq |\mathsf{seqval}\sem{y}{}^1(\pi_1', \pi_2')| <  
 	|\mathsf{seqval}\sem{y}{}^1(\pi_1, \pi_2)|\big) \Big\}
 	\end{array}
 \]
 \end{defn}
 This definition is capable to include the timing channel(control dependency) in Example~\ref{ex:excltiming},
 as well as exclude the over approximation in Example~\ref{ex:overapp}.
 %
 \begin{proof}
 \caseL{Including the Example~\ref{ex:excltiming}}
 By Example~\ref{ex:excltiming}, we have its semantics in Equation~\ref{eq:sem_timingdep}.
 %
 %
 Let $\pi_1^1, \pi_1'^1 \in \mathbb{T^{+}}$ be arbitrary traces s.t. 
 %
 $$\forall z \in \mathbb{V}\setminus \{x\}. ~ \env(\pi_1^1)(z) = \env(\pi_1'^1) $$ 
 %
 Let $v = \env(\pi_1^1)(x) $, $v' = \env(\pi_1'^1)(x')$, without lose of generalization, let $0 \leq v' < v$.
 \\
 Let 
 $t_i = {}^2 \xrightarrow{(x = x - 1) = v - i } {}^3 \xrightarrow{(y = 1) = 1} {}^1 \cdots  {}^1$, for $i = 1, \cdots, v$
 %
 $\pi_2 = {}^1 \xrightarrow{(x > 0)} {}^2 t_1 {}^1 \cdots   {}^2 t_v {}^1 \xrightarrow{\neg(x > 0)} {}^l $,
 %
  By Equation~\ref{eq:sem_timingdep}, we know:
 \[
 	\left< \pi_1^1, \pi_2 \right> \in \sem{\ewhile {}^1 (x > 0) \{{}^2 x = x - 1; {}^3 y = 1;\} }
 \]
 %
 Let 
 $t_i' = {}^2 \xrightarrow{(x = x - 1) = v' - i } {}^3 \xrightarrow{(y = 1) = 1} {}^1 \cdots  {}^1$, for $i = 1, \cdots, v'$
 %
 $\pi_2' = {}^1 \xrightarrow{(x > 0)} {}^2 t'_1 {}^1 \cdots  {}^2 t'_{v'} {}^1 \xrightarrow{\neg(x > 0)} {}^l $,
 %
  By Equation~\ref{eq:sem_timingdep}, we know:
 \[
 	\left< \pi_1'^1, \pi'_2 \right> \in \sem{\ewhile {}^1 (x > 0) \{{}^2 x = x - 1; {}^3 y = 1;\} }
 \]
 %
 \\
 By Definition of $\mathsf{seqval}$, we have:
 \[
 	|\mathsf{seqval}\sem{y}{}^1(\pi_1^1, \pi_2 )| = |\underbrace{0 \cdots 1}_{0 \leq v}| = v + 1
 \]
 %
 \[
 	|\mathsf{seqval}\sem{y}{}^1(\pi_1^1, \pi_2' )| = |\underbrace{0 \cdots 1}_{0 \leq v'}| = v' + 1
 \]
 %
 Since, $v' < v $, we have: 
 \[
 	|\mathsf{seqval}\sem{y}{}^1(\pi_1^1, \pi_2' )| < |\mathsf{seqval}\sem{y}{}^1(\pi_1^1, \pi_2 )|
 \]
 %
 Let $\Pi_2''$ defined as follows:
 \[
 	\Pi''_2 \triangleq \{
 	\left< \pi_1'^1, \pi''_2 \right> \vert
 	\pi''_2 =  {}^1 \xrightarrow{(x > 0)} {}^2 t'_1 {}^1 \cdots  {}^2 t'_{j} {}^1, \forall j < v'\} 
 \]
 %
 By Equation~\ref{eq:sem_timingdep}, we know:
 %
 \[
 		\Pi''_2 \subseteq \sem{\ewhile {}^1 (x > 0) \{{}^2 x = x - 1; {}^3 y = 1;\} }
 		\land
 		\forall \left< \pi_1', \pi''_2 \right> \in \sem{\ewhile {}^1 (x > 0) \{{}^2 x = x - 1; {}^3 y = 1;\} } 
 		\st \left< \pi_1', \pi''_2 \right> \in  \Pi''_2
 \]
 %

 %
 %
 Then for arbitrary $\left< \pi_1', \pi''_2 \right> \in \sem{\ewhile {}^1 (x > 0) \{{}^2 x = x - 1; {}^3 y = 1;\} }$, we know:
 \[
 	\exists \st \pi''_2 =  {}^1 \xrightarrow{(x > 0)} {}^2 t'_1 {}^1 \cdots  {}^2 t'_{j} {}^1 \land j \leq v'
 \]
 %
 \[
 	|\mathsf{seqval}\sem{y}{}^1(\pi_1^1, \pi_2'' )| = |\underbrace{0 \cdots 1}_{0 \leq j}| = j \leq v'
 \]
 %
 Then we have
 \[
 \begin{array}{l}
 	\forall \left< \pi_1'^1, \pi''_2 \right> \in \mathcal{S}^{+\infty} \sem{\ewhile {}^2 (x > 0) {}^3 y = 1;} \st
 	\Big(
 	|\mathsf{seqval}\sem{y}{}^1(\pi_1'^1, \pi_2'' )| \leq v' < v))\Big)
 \end{array}
 \] 
 %
 i.e.,
 \[
 	\begin{array}{l}
 	\exists \config{\pi_1, \pi_2}, \config{\pi_1', \pi_2'} \in \mathcal{S}^{+\infty}\sem{\ewhile {}^1 (x > 0) \{{}^2 x = x - 1; {}^3 y = 1;} \\
 	\quad \st \forall \config{\pi_1', \pi_2''} \in \mathcal{S}^{+\infty}\sem{\ewhile {}^1 (x > 0) \{{}^2 x = x - 1; {}^3 y = 1;} \\
 	\quad \big(
 	\forall z \in \mathbb{V}\setminus \{x\} \st \env(\pi_1)(z) = \env(\pi_1') \st \\
 	\quad  \quad  \land |\mathsf{seqval}\sem{y}{}^1(\pi_1', \pi_2'')| 
 	\leq |\mathsf{seqval}\sem{y}{}^1(\pi_1', \pi_2')| <  
 	|\mathsf{seqval}\sem{y}{}^1(\pi_1, \pi_2)|\big) 	
 	\end{array}
 \]
 \\
 %
 By modified data dependency in Definition~\ref{defn:mdfy_dep} from Definition~2 (in \cite{cousot2019abstract}), we have:
 \[
 	\mathcal{S}^{+\infty}\sem{\ewhile {}^1 (x > 0) \{{}^2 x = x - 1; {}^3 y = 1;} 
 	\in \mathcal{D}^1(x, y)
 \]
 %
 By Definition~(4) (in \cite{cousot2019abstract}), we have:
 \[
 	x \rightsquigarrow^{1}_{\ewhile {}^1 (x > 0) \{{}^2 x = x - 1; {}^3 y = 1;\}} y
 \]
 %
 \caseL{Excluding the Over Approximated Example~\ref{ex:overapp}}
 %
 Let $z \in \mathbb{V}\setminus \{x\}$ be arbitrary variable different from $x$, it is sufficient to show,
 by the modified data dependency in Definition~\ref{defn:mdfy_dep}, the following dependency cannot be derived:
 \[
 	z \rightsquigarrow^{2}_{\ewhile {}^2 (x > 0) {}^3 y = 1;} y
 \]
 Take arbitrary $\config{\pi_1, \pi_2}, \config{\pi_1', \pi_2'}$ s.t.:
 \[
 	\config{\pi_1, \pi_2}, \config{\pi_1', \pi_2'} \in \mathcal{S}^{+\infty}\sem{\ewhile {}^1 (x > 0) \{{}^2 x = x - 1; {}^3 y = 1;}  
 	\land \forall u \in \mathbb{V}\setminus \{z\} \st \env(\pi_1)(u) = \env(\pi_1')(u)
 	\]
 Then we know:
 \[
 	\env(\pi_1)(x) = \env(\pi_1')(x)
 \]
 Let $v = \env(\pi_1)(x) = \env(\pi_1')(x)$
 %
 By Definition of $\mathsf{seqval}$, we have:
 \[
 	|\mathsf{seqval}\sem{y}{}^2(\pi_1, \pi_2 )| = | 0 \cdot 1 \cdots| \leq v
 	\land
 	|\mathsf{seqval}\sem{y}{}^2(\pi_1', \pi_2' )| = | 0 \cdot 1 \cdots| \leq v
 \]
 %
 Without loss of generalization, let $\config{\pi_1', \pi_2'} \in \mathcal{S}^{+\infty}\sem{\ewhile {}^1 (x > 0) \{{}^2 x = x - 1; {}^3 y = 1;} $ s.t.
 \[
 |\mathsf{seqval}\sem{y}{}^2(\pi_1', \pi_2' )| = | 0 \cdot 1 \cdots 1| < v
 \]
 %
 There always exists $\config{\pi_1', \pi_2''} \in \mathcal{S}^{+\infty}\sem{\ewhile {}^1 (x > 0) \{{}^2 x = x - 1; {}^3 y = 1;}$ s.t.:
 \[
 	|\mathsf{seqval}\sem{y}{}^2(\pi_1', \pi_2'' )| = | 0 \cdot 1 \cdots 1| = v
 \]
 %
 Then we have:
 \[
 	\begin{array}{l}
 	\not\exists \config{\pi_1, \pi_2}, \config{\pi_1', \pi_2'} \in \mathcal{S}^{+\infty}\sem{\ewhile {}^1 (x > 0) \{{}^2 x = x - 1; {}^3 y = 1;} \\
 	\quad \st \forall \config{\pi_1', \pi_2''} \in \mathcal{S}^{+\infty}\sem{\ewhile {}^1 (x > 0) \{{}^2 x = x - 1; {}^3 y = 1;} \\
 	\quad \big(
 	\forall z \in \mathbb{V}\setminus \{x\} \st \env(\pi_1)(z) = \env(\pi_1') \st \\
 	\quad  \quad  \land |\mathsf{seqval}\sem{y}{}^1(\pi_1', \pi_2'')| 
 	\leq |\mathsf{seqval}\sem{y}{}^1(\pi_1', \pi_2')| <  
 	|\mathsf{seqval}\sem{y}{}^1(\pi_1, \pi_2)|\big) 	
 	\end{array}
 \]
 %
 By modified data dependency in Definition~\ref{defn:mdfy_dep},
 \[
 	\mathcal{S}^{+\infty}\sem{\ewhile {}^2 (x > 0) {}^3 y = 1;} 
 	\notin \mathcal{D}^2(z, y)
 \].
 %
 By Definition~(4) (in \cite{cousot2019abstract}), the following dependency cannot be derived.
 \[
 	z \rightsquigarrow^{2}_{\ewhile {}^2 (x > 0) {}^3 y = 1;} y
 \]
 %
 %
 \end{proof}
 \end{example}