\todo{
	\begin{lem}[One-on-One Mapping of vertices from $\traceG$ to $\progG$].
	\label{lem:v_trace_to_prog}
	\\
	$\traceG(\ssa{c}) = \{\traceV, \traceE\}$
	\\
	$\progG(\ssa{c}) = \{\progV, \progE, \progF\}$
\[
	\exists ~ \kw{injective} ~ f: \mathcal{AQ} \to \mathcal{AV}. 
	~ \forall \aq \in \traceV. ~ 
	f(\aq) \in \progV \land \progF(f(\aq)) = 2
\]
	\end{lem}
\begin{subproof}
Proving by Definition~\ref{def:proggraph} and Definition~\ref{def:prog_adapt}.
\end{subproof}
}
\\
\todo{
	\begin{lem}[One-on-One Mapping from $\edges$ of $\traceG$ to $\paths(\progG)$].
	\label{lem:bie_trace_to_prog}
	\\
	$\traceG(\ssa{c}) = \{\traceV, \traceE\}$
	\\
	$\progG(\ssa{c},\ssa{m},\text{D}) = \{\progV, \progE, \progF\}$
	\\
	An injective function $ f: \traceV \to \progV$ s.t.,
	$\forall \aq \in \traceV. ~ \progF(f(\aq)) = 2$ 
\[
	\forall e = (\aq_1, \aq_2) \in \traceE. ~ 
	\exists p_{f(\aq_1) \to f(\aq_2)} \in \paths(\progG(\ssa{c}, \text{D}, \ssa{m}))
\]
	\end{lem}
\begin{subproof}
Proving by Lemma~\ref{lem:injv_trace_to_prog} and Definition~\ref{def:proggraph} and acyclic property of $\traceG$ and $\progG$.
\end{subproof}
}
\\
\todo{
	\begin{lem}[Surjective Mapping of Vertices from $\progG$ to $\progG$].
	\label{lem:sujv_prog_to_prog}
	\\
	$\progG(\ssa{c},\ssa{m},\text{D}) = \{\progV, \progE, \progF\}$
	\\
	$\progG(\ssa{c}) = \{\progV, \progE, \progF, \progW\}$
	\\
	$\exists ~ \kw{surjective} ~ f: \mathcal{AV} \to \mathcal{SVAR}.$
	%
\[
	\forall \av \in \progV. ~ 
	f(\av) \in \progV \land \progF(f(\av)) = \progF(\av) \land
	|\kw{image}(f(\av))| \leq W(f(\av))
\]
\end{lem}
\begin{subproof}
Proving by Definition~\ref{def:proggraph}.
\end{subproof}
}
\\
\todo{
	\begin{lem}[Surjective Mapping from $\edges$ of $\progG)$ to $\edges$ of $\progG$].
	\label{lem:suje_prog_to_prog}
	\\
	$\progG(\ssa{c},\ssa{m},\text{D}) = \{\progV, \progE, \progF\}$
	\\
	$\progG(\ssa{c}) = \{\progV, \progE, \progF, \progW\}$
	\\
	A surjective function $f: \progV \to \progV$ s.t.,
	$\forall \av \in \progV. ~ \progF(f(\av)) = \progF(\av) \land |\kw{image}(f(\av))| \leq W(f(\av))$
	%
\[
	\exists ~ \kw{surjective} ~ g: \progE \to \progE. ~
	\forall e_{prog} = (\av_1, \av_2) \in \progE. 
	\exists e_{prog} = ({f(\av_1), f(\av_2)}) \in \progE
\]
\end{lem}
\begin{subproof}
Proving by Lemma~\ref{lem:sujv_prog_to_prog}.
\end{subproof}
}
\\
\todo{
	\begin{lem}[Surjective Mapping from $\paths(\progG)$ to $\walks(\progG)$].
	\label{lem:sujpathwalk_prog_to_prog}
	\\
	$\progG(\ssa{c},\ssa{m},\text{D}) = \{\progV, \progE, \progF\}$
	\\
	$\progG(\ssa{c}) = \{\progV, \progE, \progF, \progW\}$
	\\
	A surjective function $f: \progV \to \progV$ s.t.,
	$\forall \av \in \progV. ~ \progF(f(\av)) = \progF(\av) \land |\kw{image}(f(\av))| \leq W(f(\av))$
	\\
	A surjective function $g: \progE \to \progE$ s.t.,
	$\forall e_{prog} = (\av_1, \av_2) \in \progE. 
	\exists e_{prog} = ({f(\av_1) \to f(\av_2)}) \in \progE$
	\\
	$\exists ~ \kw{surjective} ~ h: \paths(\progG(\ssa{c},\ssa{m},\text{D})) \to \walks(\progG(\ssa{c}))$ s.t.:
	%
\[
	\forall p_{\av_1 \to \av_2} \in \paths(\progG(\ssa{c},\ssa{m},\text{D}))
	\text{ with }
	\left\{
	\begin{array}{ll}
	\mbox{edge sequence:} & (e, \ldots, e_{n-1})
	\\ 
	\mbox{vertices sequence:} & (\av_1, \ldots, \av_n)
	\end{array}
	\right.
\]
\[
	\exists k_{f(\av_1) \to f(\av_2)} \in \walks(\progG(\ssa{c}))
	\text{ with }
	\left\{
	\begin{array}{ll}
	\mbox{edge sequence:} & (g(e), \ldots, g(e_{n-1}) 
	\\ 
	\mbox{vertices sequence:} & (f(\av_1), \ldots, f(\av_{n}))
	\end{array}
	\right.
\]
% \item $(e, \ldots, e_{n-1})$, $(\av_1, \ldots, \av_n)$ are the edges sequence and vertices sequence of $p_{\av_1 \to \av_2}$.
% then, 
%  $\len(p_{\av_1 \to \av_2}) = \len(k_{f(\av_1) \to f(\av_2)})$
% %
% \item $\forall \av \in p_{\av_1 \to \av_2}. ~ f(\av) \in k_{f(\av_1) \to f(\av_2)}$
% %
% \item $\forall \av \in p_{\av_1 \to \av_2}. ~ 
% \kw{image}(f(\av)) \cap {p_{\av_1 \to \av_2}}| = \# \{f(\av) \prog f(\av) \in k_{f(\av_1) \to f(\av_2)}\}
% $
\end{lem}
%
\begin{subproof}
Proving by induction on the length of $l = p_{\av_1 \to \av_2} \in \paths(\progG(\ssa{c},\ssa{m},\text{D}))$, and Lemma~\ref{lem:suje_prog_to_prog} and Lemma~\ref{lem:sujv_prog_to_prog}.
\caseL{ $l = 1$: }
\caseL{ $l = l' + 1$, $l' \geq 1$: }
\end{subproof}
}
\end{proof}
%
%
%
}